test/coq/records_proof.v
@@ -10,57 +10,88 @@ From test Require Import records.
 
 Local Transparent eval. (* TODO. *)
 
+(* -------------------------------------------------------------------------- *)
+
 Context `{!osirisGS_gen hlc Σ}.
 
-Definition enc_r_elt : val :=
-  VRecord $
-          EnvCons "b" (encode true) $
-          EnvCons "i" (encode 10) $
-          EnvNil.
-Definition enc_r_elt' : val :=
-  VRecord $
-          EnvCons "b" (encode false) $
-          EnvCons "i" (encode 10) $
-          EnvNil.
+(* -------------------------------------------------------------------------- *)
 
+(* Local defintiion of the record type used in [records.ml]. *)
+
+Record R :=
+  { b: bool ;
+    i: Z }.
+
+Local Instance r_encode : Encode R :=
+  { encode :=
+    fun (r: R) =>
+      VRecord $
+              EnvCons "b" #(r.(b)) $
+              EnvCons "i" #( r.(i)) $
+              EnvNil }.
+
+(* -------------------------------------------------------------------------- *)
+
+(* Definition of some values; useful to write the specs below. *)
+Definition enc_r_elt : val := #{| b := true; i := 10 |}.
+Definition enc_r_elt' : val := #{|b := false; i := 10|}.
 Definition enc_lily : val := # [enc_r_elt; enc_r_elt'].
 
+(* -------------------------------------------------------------------------- *)
+
+(* Definition of the specifications. *)
+
+(* [is_equal] asserts the equality of two values. *)
 Definition is_equal v : val → iProp Σ :=
   λ res, ⌜ res = v ⌝%I.
 
-Definition flip_spec (v : val) : iProp Σ :=
-  ∀ (v': val) (b: bool) (i: Z),
-    is_equal v' (VRecord $
-                         EnvCons "b" (encode b) $
-                         EnvCons "i" (encode i) $
-                         EnvNil) -∗
-    WP call v v'
-    {{ λ r, is_equal r (VRecord $
-                                EnvCons "b" (encode (negb b)) $
-                                EnvCons "i" (encode i) $
-                                EnvNil) }}.
-
-Definition r_val_spec (r_val: val): iProp Σ :=
-  ∀ (r: val) (i: Z) (b: bool),
-    ⌜ r = VRecord $
-                  EnvCons "b" #b $
-                  EnvCons "i" #i $
-                  EnvNil ⌝ →
-    WP call r_val r {{ λ result,
-    match b with
-    | true => ⌜ result = #(i * 2 - 1)%Z ⌝
-    | false => ⌜ result = # i ⌝
-    end }}.
-
+(* [trivial_spec] is a dummy specification. *)
 Definition trivial_spec (v: val) : iProp Σ :=
   ⌜ True ⌝.
+
+(* [flip] negates [b] in records of type [{ b: bool; i: int}]. *)
+Definition flip_spec (v : val) : iProp Σ :=
+  ∀ (b: bool) (i: Z),
+    WP call v #{| b := b; i := i |}
+    {{ λ r, is_equal r #{| b := negb b; i := i |} }}.
+
+(* [r_val_spec] performs a different arithmetic computation depending on the
+   fiels [b] of a record. *)
+Definition r_val_pure (r: R) : Z :=
+  match r.(b) with
+  | true => r.(i) * 2 - 1
+  | false => r.(i)
+  end.
+
+Definition r_val_spec (r_val: val): iProp Σ :=
+  ∀ (i: Z) (b: bool),
+    let r := {| b := b; i := i |} in
+    WP call r_val #r
+       {{ λ result, is_equal result #(r_val_pure r) }}.
+
+Definition sum_pure (r1 r2: R) : Z :=
+  r_val_pure r1 + r_val_pure r2.
+Definition sum_spec (vsum: val) : iProp Σ :=
+  ∀ (b1 b2: bool) (i1 i2: Z),
+    let r1 := {| b := b1; i := i1 |} in
+    let r2 := {| b := b2; i := i2 |} in
+    WP call vsum #r1 {{
+          λ vpart,
+          WP call vpart #r2 {{
+                λ res,
+                is_equal res # (sum_pure r1 r2) }} }}.
+
+(* -------------------------------------------------------------------------- *)
+
+(* Proof of the module [Records] in which the function bodies have not been
+   turned opaque. *)
 
 Lemma Records_spec :
     let Λ :=
       [
         ("is_odd", trivial_spec) ;
         ("is_odd_naive", trivial_spec) ;
-        ("sum", trivial_spec) ;
+        ("sum", sum_spec) ;
         ("r_val", r_val_spec) ;
         ("lily", is_equal enc_lily) ;
         ("flip", flip_spec) ;
@@ -71,4 +102,406 @@ Lemma Records_spec :
            EnvNil in
   ⊢ WP eval_mexpr η Records {{ module_spec Λ }}.
 Proof.
-Admitted.
+  intros Λ η. wp.
+  simpl (build _ _). wp.
+
+  (* [r_elt] is a known value. *)
+  wp_specify "r_elt" (is_equal enc_r_elt); first done.
+  (* There is no need to keep the "spec" of [r_elt] around.*)
+  iIntros (r_elt) "->". wp_continue.
+
+  (* [flip] has the expected spec. *)
+  wp_specify "flip" flip_spec.
+  { iIntros (b i); wp_call.
+    wp_continue. simpl (build _ _). wp. done. }
+  iIntros (flip) "#Hflip". wp_continue.
+
+  (* [flip] is applied to [r_elt]. *)
+  replace
+    (VRecord (EnvCons "b" VTrue (EnvCons "i" (VInt (int.repr 10)) EnvNil)))
+    with #{| b := true; i := 10 |}; last reflexivity.
+  wp_use "Hflip".
+  iIntros (? <-). wp.
+
+  (* [lily] has the expected value. *)
+  wp_specify "lily" (is_equal enc_lily).
+  { iPureIntro. reflexivity. }
+  iIntros (lily) "#Hlily". wp_continue.
+
+
+  (* TODO: uncomment the call to [List.rev]. *)
+
+  (* [r_val] has the expected value. *)
+  wp_specify "r_val" r_val_spec.
+  { iIntros (i [|]).
+    (* Case: [b] is true. *)
+    { wp_call. by do 2 wp_continue. }
+    { wp_call. by do 2 wp_continue. } }
+  iIntros (r_val) "#Hr_val". wp_continue.
+
+
+  (* [sum] is given the trivial spec for now. *)
+  wp_specify "sum" sum_spec.
+  { iIntros(b1 b2 i1 i2). wp_call. do 2 wp_continue.
+    wp.
+    wp_par.
+    2: by wp_use "Hr_val".
+    { wp_use "Hr_val". iIntros(?<-).
+      apply tc_change_goal. iIntros (vpartial).
+      iIntros "H"; iExact "H". }
+    { iIntros (v1 v2) "Hadd <-".
+      wp. iApply (wp_covariant with "Hadd").
+      iIntros (?->). iPureIntro. reflexivity. } }
+  iIntros (sum) "#Hsum". wp_continue.
+
+  (* [is_odd_naive] is given the trivial spec for now. *)
+  wp_specify "is_odd_naive" trivial_spec; first done.
+  iIntros (is_odd_naive) "#His_odd_naive". wp_continue.
+
+  (* [is_odd] is given the trivial spec for now. *)
+  wp_specify "is_odd" trivial_spec; first done.
+  iIntros (is_odd) "#His_odd". wp_continue.
+
+  (* TODO: uncomment the calls to [sum] and [List.fold_left] *)
+
+  (* Every spec has been proven: [wp_module_spec] can finish the proof. *)
+  wp_module_spec.
+Time Qed.
+
+(* -------------------------------------------------------------------------- *)
+
+(* Definition of function bodies.  These are the bodies of functions which will
+   be proven. The goal is to see if it is easier to specify each of these bodies
+   before the main proof. *)
+
+(* Body of [flip]. *)
+Definition flip_body (r: var) :expr :=
+  ERecordUpdate (EPath (PathBase r))
+                (FECons
+                   "b"
+                   (EApp (EPath (PathDot (PathBase "Stdlib") "not"))
+                         (ERecordAccess (EPath (PathBase r)) "b")) FENil).
+
+Definition is_odd_body : expr :=
+  EApp
+    (EApp (EPath (PathDot (PathBase "Stdlib") "=")) $
+          EApp (
+            EApp (EPath (PathDot (PathBase "Stdlib")
+                                 "mod")) $
+                 EPath (PathBase "n"))
+          (EInt 2))
+    (EInt 0).
+
+Definition is_odd_naive_body : expr :=
+  ESeq
+    (EAssert $
+             EApp
+             (EApp (EPath (PathDot (PathBase "Stdlib") ">="))
+                   (EPath (PathBase "n"))) $
+             EInt 0) $
+    EIfThenElse (
+      EApp
+        (EApp (EPath (PathDot (PathBase "Stdlib") ">"))
+              (EPath (PathBase "n")))
+        (EInt 1))
+    (EApp (EPath (PathBase "is_odd_naive")) $
+          EApp
+          (EApp (EPath (PathDot (PathBase "Stdlib")
+                                "-"))
+                (EPath (PathBase "n")))
+          (EInt 2)) $
+    EIfThenElse (
+      EApp (
+          EApp (EPath (PathDot (PathBase "Stdlib")
+                               "="))
+               (EPath (PathBase "n")))
+           (EInt 0))
+    (EData "false" (ETuple ENil))
+    (EData "true" (ETuple ENil))
+.
+
+Definition sum_body : expr :=
+  EApp (
+      EApp (EPath (PathDot (PathBase "Stdlib") "+")) $
+           EApp (EPath (PathBase "r_val"))
+           (EPath (PathBase "r1"))
+    ) $
+       EApp (EPath (PathBase "r_val"))
+       (EPath (PathBase "r2"))
+.
+Definition r_elt_body : expr :=
+  ERecord (
+      FECons "i"
+             (EInt 10)
+              (FECons "b" (EData "true" (ETuple ENil)) FENil)).
+
+Definition lily_body : expr :=
+  EData "::"
+        $ ETuple  $
+        ECons (EPath (PathBase "r_elt")) $
+        ECons
+        (EData "::"
+               (ETuple $
+                       ECons (
+                         EApp (EPath (PathBase "flip"))
+                              (EPath (PathBase "r_elt"))) $
+                       ECons (EData "[]" (ETuple ENil))
+                       ENil))
+        ENil
+.
+
+Definition r_val_body (r: var) : expr :=
+  EMatch (ERecordAccess (EPath (PathBase r)) "b") $
+         MkBranches
+         [ Branch (PBool true) $
+                  EApp (
+                    EApp (EPath (PathDot (PathBase "Stdlib") "-"))
+                         (EApp (
+                              EApp (EPath (PathDot (PathBase "Stdlib")
+                                                   "*"))
+                                   (ERecordAccess (EPath (PathBase r)) "i")
+                            )
+                               (EInt 2)
+                         )
+                  )
+                  (EInt 1)
+           ; Branch (PBool false)
+                    (ERecordAccess (EPath (PathBase r)) "i")
+         ]
+.
+
+Definition Opacified_Records : mexpr :=
+  MkStruct [
+      ILet (Binding1 (PVar "r_elt") r_elt_body)
+      ;
+      ILet (Binding1 (PVar "flip")
+                     (EAnonFun (
+                          AnonFun1Pat (PVar "r")
+                                      (flip_body "r"))))
+      ;
+      ILet (Binding1 (PVar "lily") lily_body)
+      ;
+      ILet $
+          Binding1 (PVar "r_val") $
+                   EAnonFun ( AnonFun1Pat (PVar "r") (r_val_body "r"))
+      ;
+      ILet $
+           Binding1 (PVar "sum") $
+           EAnonFun $
+           AnonFun1Pat (PVar "r1") $
+           EAnonFun $
+           AnonFun1Pat (PVar "r2") $
+           sum_body
+      ;
+      ILetRec $
+          RecBiCons
+          (RecBinding "is_odd_naive" $
+           AnonFun1Pat (PVar "n") $
+           is_odd_naive_body)
+          RecBiNil
+      ;
+      ILet $
+           Binding1 (PVar "is_odd") $
+           EAnonFun $
+           AnonFun1Pat (PVar "n") $
+           is_odd_body
+    ].
+
+Lemma Records_eq :
+  Records =
+    Opacified_Records.
+Proof. reflexivity. Qed.
+
+
+(* Bodies are turned opaque. *)
+Opaque
+  flip_body
+  lily_body
+  is_odd_body
+  is_odd_naive_body
+  r_val_body
+.
+
+(* -------------------------------------------------------------------------- *)
+
+(* Specifications of function bodies. *)
+
+Lemma flip_body_spec :
+  ∀ (r: var) (b: bool) (i: Z) η,
+    lookup_name η "Stdlib" = ret Stdlib →
+    lookup_name η r = ret #{| b := b; i := i |} →
+    simp (eval η (flip_body r))
+         (ret #{| b := negb b; i := i |}).
+Proof.
+  with_strategy transparent [flip_body] unfold flip_body.
+  intros r [] i η Hstdlib Hr; simp;
+    (eapply prove_simp_bind;
+     [ with_strategy transparent [ Stdlib__not ] unfold Stdlib__not;
+       with_strategy transparent [ call ] unfold call; simp
+     | simp ]).
+Qed.
+
+Lemma lily_body_spec η η' :
+  let clo_flip := VClo η' (AnonFun1Pat (PVar "r") (flip_body "r")) in
+  (* Thefollowing is required to use [flip_body_spec]. *)
+  lookup_name η' "Stdlib" = ret Stdlib →
+  lookup_name η "r_elt" = ret enc_r_elt →
+  lookup_name η "flip" = ret clo_flip →
+  lookup_name η "Stdlib" = ret Stdlib →
+  simp (eval η lily_body) (ret enc_lily).
+Proof.
+  intros ? ? Hrelt Hflip Hstdlib.
+  with_strategy transparent [lily_body] unfold lily_body.
+  simp.
+  rewrite Hrelt; simp.
+  eapply prove_simp_bind.
+  { with_strategy transparent [call] unfold call.
+    simpl. simp.
+    with_strategy transparent [ concatenating ] (unfold concatenating at 1).
+    eapply flip_body_spec; try done.
+    (* FIXME. *)
+    instantiate (1 := 10). instantiate (1 := true).
+    done. }
+  simp.
+Qed.
+
+Ltac rew name :=
+  with_strategy transparent [ name ] unfold name.
+
+Arguments String.eqb !s1 !s2 : simpl nomatch. (* TODO *)
+Lemma r_val_body_spec η (r: R) (rvar: var) :
+  lookup_name η "Stdlib" = ret Stdlib →
+  lookup_name η rvar = ret #r →
+  simp (eval η (r_val_body rvar)) (ret #(r_val_pure r)).
+Proof.
+  rew r_val_body.
+  intros??. destruct (r.(b)) eqn:E;
+    simp; rewrite E; simp; simp_continue;
+    rewrite /r_val_pure E; simp.
+  rew Stdlib__mul. rew Stdlib__sub. rew call.
+  simp.
+  rewrite int.mul_repr_repr
+          int.sub_repr_repr.
+  simp.
+Qed.
+
+Lemma sum_body_spec η (r1 r2: R):
+  lookup_name η "Stdlib" = ret Stdlib →
+  simp (eval η sum_body) (ret #(sum_pure r1 r2)).
+Proof.
+  intros?.
+  rew sum_body.
+  simp. Admitted.
+
+(* -------------------------------------------------------------------------- *)
+
+(* [wp] and [wp_continue] do *not* respect the opacity of the above expressions.
+   This is caused by [apply tc_change_goal] in [wp]which tries to simplify the
+   goal using any instance of [TC_change_goal]. *)
+
+Ltac wp' := wp.
+Ltac wp'_continue := wp_continue.
+
+Ltac wp :=
+  iStartProof; cbn;
+   repeat
+    lazymatch goal with
+    | |- environments.envs_entails _ (▷ _) => iNext
+    | _ => wp_step; try progress cbn
+    end.
+
+Ltac wp_continue :=
+  lazymatch goal with
+  | |- environments.envs_entails
+         _ (wp _ _ (concatenating eval _ _ ?δ) _) =>
+      with_strategy transparent [ concatenating ] (unfold concatenating at 1)
+  | |- environments.envs_entails
+         _ (wp _ _ (dconcatenating ?δ _) _) =>
+      with_strategy transparent [ dconcatenating ] (unfold dconcatenating at 1)
+  end; wp.
+
+Ltac wp_simp_using H :=
+  iApply wp_simp; [ by apply H | wp ].
+
+Lemma Records_spec_bodies :
+    let Λ :=
+      [
+        ("is_odd", trivial_spec) ;
+        ("is_odd_naive", trivial_spec) ;
+        ("sum", sum_spec) ;
+        ("r_val", r_val_spec) ;
+        ("lily", is_equal enc_lily) ;
+        ("flip", flip_spec) ;
+        ("r_elt", is_equal enc_r_elt)
+    ]
+  in
+  let η := EnvCons "Stdlib" Stdlib $
+           EnvNil in
+  ⊢ WP eval_mexpr η Records {{ module_spec Λ }}.
+Proof.
+  rewrite Records_eq.
+
+  (* Proof using [simp]. *)
+  intros ??. wp.
+  simpl (build _ _). wp.
+
+  wp_specify "r_elt" (is_equal enc_r_elt); first done.
+  iIntros(?->). wp_continue.
+
+  wp_continue.
+  iApply wp_simp.
+  { by eapply lily_body_spec; try done. }
+
+  wp. wp_continue.
+
+  (* [r_val] has the expected value. *)
+  wp_specify "r_val" r_val_spec.
+  { iIntros (i[|]).
+    (* Case: [b] is true. *)
+    { wp_call. wp'_continue.
+      iApply wp_simp; first eapply r_val_body_spec.
+      - done.
+      - by instantiate (1 := {| b := true; i := i |}).
+      - by wp. }
+    { wp_call. wp'_continue.
+      iApply wp_simp; first eapply r_val_body_spec.
+      - done.
+      - by instantiate (1 := {| b := false; i := i |}).
+      - by wp. } }
+  iIntros (r_val) "#Hr_val". wp_continue.
+
+
+  (* [sum] is given the trivial spec for now. *)
+  wp_continue.
+
+  (* [is_odd_naive] is given the trivial spec for now. *)
+  wp_specify "is_odd_naive" trivial_spec; first done.
+  iIntros (is_odd_naive) "#His_odd_naive". wp_continue.
+
+  (* [is_odd] is given the trivial spec for now. *)
+  wp_specify "is_odd" trivial_spec; first done.
+  iIntros (is_odd) "#His_odd". wp_continue.
+
+
+  lazymatch goal with
+  | |- environments.envs_entails _ (?φ (VStruct ?η)) =>
+      iExists _; iSplit ; first (iPureIntro; reflexivity)
+  end.
+  cbn; repeat iSplitL; try (iExists _; iSplit; first done); try done.
+  { (* Proof of the [sum] function.*)
+    iIntros(b1 b2 i1 i2).
+    wp_call. wp_continue. wp_continue.
+    wp_par.
+    - wp_use "Hr_val".
+      iIntros(?<-).
+      wp_call. wp_set_postcondition.
+    - wp_use "Hr_val".
+    - iIntros (v1 v2 -> <-). wp.
+      wp_call.
+      iPureIntro. unfold sum_pure;
+        destruct b1, b2; cbn;
+        by rewrite int.add_repr_repr. }
+  { (* Proof of the [flip] function. *)
+    iIntros(??); wp_call. wp_continue.
+    by wp_simp_using flip_body_spec. }
+Time Qed.
